Quave/env.lean
@@ -2,33 +2,51 @@ import Quave.Basic
 
 open qwhilep
 
-/-- A context in which the program evaluates its variables and expressions-/
+/-
+A context in which the program evaluates its variables and expressions
+-/
 def Env := String → Value
 
 
+/-
+Namespace: Env
+-/
 namespace Env
 
-/-- Set a value in an environment -/
+/-
+Set a value in an environment
+-/
 def set (x : String) (v : Value) (σ : Env) : Env :=
   fun y => if x == y then v else σ y -- If x == y, return v, else return σ y
 
-/-- Look up a value in an environment -/
+/-
+Look up a value in an environment
+-/
 def get (x : String) (σ : Env) : Value :=
   σ x -- Return the value of x in σ
 
-/-- Initialize an environment, setting all uninitialized memory to `i` -/
-def init (i : Value) : Env := fun _ => i -- Return i for all variables
+/-
+Initialize an environment, setting all uninitialized memory to `i`
+-/
+def init (i : Value) : Env :=
+  fun _ => i -- Return i for all variables
 
-/-- Initialize an environment with all memory set to 0 -/
+/-
+Initialize an environment with all memory set to 0
+-/
 @[simp]
 theorem get_init (v : Value) (x : String) : (Env.init v).get x = v := by rfl
 
-/-- Set a value in an environment, then look it up -/
+/-
+Set a value in an environment, then look it up
+-/
 @[simp]
 theorem get_set_same (v : Value) (x : String) {σ : Env} : (σ.set x v).get x = v := by
   simp [get, set]
 
-/-- Set a value in an environment, then look up a different value -/
+/-
+Set a value in an environment, then look up a different value
+-/
 @[simp]
 theorem get_set_different (v : Value) (x y : String) {σ : Env} : x ≠ y → (σ.set x v).get y = σ.get y := by
   intros
@@ -37,21 +55,46 @@ theorem get_set_different (v : Value) (x y : String) {σ : Env} : x ≠ y → (�
 end Env
 
 
-
-
-
+/-
+Namespace: ClassicalExpr
+-/
 namespace ClassicalExpr
 
-/-- Evaluate a classical expression in an environment.
-    Returns `none` if the expression contains an undefined variable.
-    Otherwise, returns `some v`, where `v` is the value of the expression.
-    -/
+/-
+Evaluate a classical expression in an environment.
+  Returns `none` if the expression contains an undefined variable.
+  Otherwise, returns `some v`, where `v` is the value of the expression.
+-/
 def eval (σ : Env) : ClassicalExpr → Option Value
   | .const i => some i
-  | .var x => σ.get x
+  | .var x => σ.get x -- Does get x return Option Value?
   | .add e₁ e₂ =>
       match (eval σ e₁, eval σ e₂) with
       | (some v₁, some v₂) => some (v₁ + v₂)
       | _ => none
+  | .sub e₁ e₂ =>
+      match (eval σ e₁, eval σ e₂) with
+      | (some v₁, some v₂) => some (v₁ - v₂)
+      | _ =>
+  | .mul e₁ e₂ =>
+      match (eval σ e₁, eval σ e₂) with
+      | (some v₁, some v₂) => some (v₁ * v₂)
+      | _ => none
 
 end ClassicalExpr
+
+
+/-
+Namespace: BooleanExpr
+-/
+namespace BooleanExpr
+
+/-
+Evaluate a boolean expression in an environment.
+  Returns `none` if the expression contains an undefined variable.
+  Otherwise, returns `some v`, where `v` is the value of the expression.
+-/
+def eval (σ : Env) : BooleanExpr → Option Bool
+  | .True =>
+
+end BooleanExpr
